##### 1 求证：$I_{\lambda}(s,z)=I_{\lambda}(0)e^{-\sec z \tau_{\lambda t}}$
证明：已知
$$
dI_\lambda=-\kappa_\lambda\cdot I_\lambda ds\tag{1}
$$
两边同除$I_\lambda$并积分可得
$$\begin{align}
\Delta(\ln I_\lambda)=\ln I_\lambda(s)-\ln I_\lambda(0)=-\int_s^{\lambda}k_{\lambda}ds=-\int_0^\tau(s)d\tau_\lambda=-\tau_\lambda(s)\tag{2}\\
\end{align}
$$
对最右侧式子取对数，得
$$\begin{align}
\ln I_\lambda(s)&=\ln I_\lambda(0)-\ln e^{\tau(s)}\\
\ln I_\lambda(s)&=\ln I_\lambda(0)e^{-\tau_\lambda(s)}\\\tag{3}
I_\lambda(s)&=I_\lambda(0)e^{-\tau_\lambda(s)}
\end{align}
$$
由于$$
\sec z=\frac{s}{t}=\frac{ds}{dt}\tag{4}
$$
故$$
ds=\sec zdt\tag{5}
$$
因此$$
\tau_{\lambda}(s)=\int_0^s \kappa_\lambda ds=\sec z\int_0^t\kappa_\lambda dt=\sec z\tau_{\lambda t}\tag{6}
$$
带入（3）式，可得$$
I_\lambda(s,z)=I_\lambda(0)e^{-\sec z \tau_{\lambda t}}
$$